\documentclass[12pt,russian]{article}
\renewcommand{\baselinestretch}{1}
%\renewcommand{\baselinestretch}{1.5}
\textwidth=158mm
\textheight=232mm
\voffset=-24mm
%\pagestyle{empty}

\usepackage[russian]{babel}
\usepackage{amsmath,amssymb,amsthm,amsfonts}
\usepackage{multirow}
\newcommand{\Real}{\mathbb R}
\newcommand{\Nat}{\mathbb N}
\newcommand{\norm}[1]{\left\Vert#1\right\Vert}
\newcommand{\abs}[1]{\left\vert#1\right\vert}
\newcommand{\bignorm}[1]{\bigl\Vert#1\bigr\Vert}
\newcommand{\bigabs}[1]{\bigl\vert#1\bigr\vert}
\newcommand{\set}[1]{\left\{#1\right\}}
\renewcommand{\phi}{\varphi}
\newcommand{\eps}{\varepsilon}
\renewcommand{\ge}{\geqslant}
\renewcommand{\le}{\leqslant}
\renewcommand{\liminf}{\underline{\lim}}
\newcommand{\grad}{\triangledown}
\newcommand{\card}{{\rm card}}
\newtheorem{thm}{Theorem}
\newtheorem{prop}{Proposition}
\newtheorem{lm}{Lemma}
\newtheorem{rem}{Remark}
\newtheorem{cor}{Corollary}
\newcommand{\To}{\longrightarrow}
\newcommand{\Wf}{\stackrel{o\ }{W_1^1}}
\newcommand{\W}{W_1^1}
\newcommand{\sign}{\mathop{\rm sign}\nolimits}
\newcommand{\dist}{\mathop{\rm dist}\nolimits}
\newcounter{pictureCounter}
\begin{document}

\title{On monotonicity of some functionals under rearrangements}
\author{
S.~Bankevich\\
\texttt{Sergey.Bankevich@gmail.com}
\and
A.~Nazarov\\
\texttt{al.il.nazarov@gmail.com}
}

\maketitle

\section{Introduction}

First, we recall the layer cake representation for a measurable function $u: [-1, 1] \to \Real_+$
(here and elsewhere $\Real_+ = [0,\infty)$).
Namely, if we set $\mathcal{A}_t: = \{x \in [-1,1]:\ u(x)> t \}$
then $u(x) = \int_0^\infty \chi_{\mathcal{A}_t}dt$.

We define the monotone rearrangement of a measurable set $E \subset [-1, 1]$ and the
monotone rearrangement of non-negative function $u \in \W (-1, 1)$ as follows:
\begin{eqnarray*}
E^*: = [1 - \abs{E}, 1] \qquad
u^*(x): = \int_0^\infty \chi_{\mathcal{A}_t^*}dt
\end{eqnarray*}

Under the same conditions we define the symmetric rearrangement 
(symmetrization) for sets and functions:
\begin{eqnarray*}
\overline{E} := [-\frac{\abs{E}}{2}, \frac{\abs{E}}{2}] \qquad
\overline{u}(x) := \int_0^\infty \chi_{\overline{\mathcal{A}_t}}dt
\end{eqnarray*}

We denote by $\mathfrak{F}$ the set of continuous functions 
$F: \Real_+ \times \Real_+ \to \Real_+,$
which are convex and increasing with respect to the second argument.

Let us consider a functional
\begin{equation}
\label{functional}
I(a, u) = \int_{-1}^1 F(u(x), a(x, u(x)) \abs{u'(x)}) dx,
\end{equation}
where $a: [-1, 1] \times \Real_+ \to \Real_+$ is a continuous function, $F \in \mathfrak{F}$.

It is well known that if $a \equiv const$ then the inequalities
\begin{eqnarray}
\label{toprove}
I(a, u^*) & \le & I(a, u), \qquad \qquad u \in \W(-1, 1);\\
\label{toproveSymm}
I(a, \overline{u}) & \le & I(a, u), \qquad \qquad u \in \Wf(-1, 1)
\end{eqnarray}
hold, see for example \cite{Kawohl} and references therein.

The inequality (\ref{toproveSymm}) and its multi-dimensional analogue
are proved in \cite{Br} provided that the function $a$ is even and convex 
with respect to $x$. However, the proof contains a gap,
and in fact this inequality was proved in \cite{Br} only for Lipschitz functions $u$.

Namely, while proving the inequality (\ref{toproveSymm}) for a natural class of functions,
the author of \cite{Br} approximates $u \in \Wf$ having finite integral (\ref{functional})
using piecewise linear functions $u_k$ and claims that $I(a, u_k) \to I(a, u)$.
However, this assertion is not justified and in general is is not true.
In 1926, M.~A.~Lavrentiev proposed the first example of an integral functional
for which the infimum over the domain is strictly less than the infimum over the set of 
Lipschitz functions. For historical overview and simple examples of ``one-dimensional'' 
functionals for which the Lavrentiev phenomenon takes place see, e.g., \cite{BGH}.
Note that a deep investigation of the Lavrentiev phenomenon for some classes of multidimensional 
functionals was realized by V.~V.~Zhikov (see, e.g., \cite{Zh1}, \cite{Zh2}).

In the paper \cite{ASC} the absence of the Lavrentiev phenomenon was proved for the functionals
$I(a, u) = \int_{-1}^1 F(u, u')$. Moreover it was shown that for every $u \in \W(-1, 1)$ 
there exists a sequence of Lipschitz functions $u_k$, such that
\begin{equation}
\label{convergence}
u_k \to u \text{ in } \W (-1, 1) \quad \text{ and } \quad I (a, u_k) \to I (a, u).
\end{equation}

We modify the proof from \cite{ASC} and prove the absence of the Lavrentiev phenomenon
for the functionals of the form (\ref{functional}).
This allows us fill a gap in the proof from \cite{Br} in one-dimensional case.
In addition we prove that evenness and convexity of the weight is a necessary condition
for the inequality (\ref{toproveSymm}) to hold.

The bulk of our paper is devoted to the inequality (\ref{toprove}).
We find a necessary and sufficient condition on the weight $a$ for the inequality 
(\ref{toprove}) to hold%
\footnote{In particular, the inequality is satisfied if the weight function $a$ is even 
and concave in $x$.}.
Under certain additional assumptions this result was announced in \cite{DAN}.

We note also that the inequality (\ref{toprove}) was considered in \cite{Lan}
for functionals similar to (\ref{functional}) under additional constraint $u(-1) = 0$.
We obtain necessary and sufficient conditions for (\ref{toprove}) under this constraint.
(The author of \cite{Lan} assumed that the weight $a$ was decreasing in $x$.)

The article is divided into 8 sections.
In Section 2 we deduce the assumptions on the weight function $a$ which are necessary for the 
inequality (\ref{toprove}).
In \S3 auxiliary statements for weights satisfying necessary conditions are established.
In \S4 the inequality (\ref{toprove}) is proved for piecewise linear functions $u$.
In \S5 we present the scheme for proving inequality (\ref{toprove}) for a wider class of 
functions $u$.
In \S6 we prove inequality (\ref{toprove}), provided that the weight $a$ first increases, 
then decreases.
\S7 is devoted to the proof of (\ref{toprove}) under necessary conditions only.
Finally, in the \S8 we consider the case of symmetric rearrangement.
There we obtain necessary conditions on the weight and complete the proof of (\ref{toproveSymm}).

\section{ The conditions necessary for the inequality (\ref{toprove})}

\begin{thm}
{\bf 1}. Let the inequality (\ref{toprove}) hold for some $F \in \mathfrak {F}$
and arbitrary piecewise linear $u$. Then the weight function $a$ is even with respect to the first argument,
that is $a(x, v) \equiv a(-x, v)$.

{\bf 2}. Let the inequality (\ref{toprove}) hold for arbitrary $F \in \mathfrak{F}$
and arbitrary piecewise linear $u$. Then the weight function $a$ satisfies
\begin{equation}
\label{almostConcave}
a(s, v) + a(t, v) \ge a(1 - t + s, v), \qquad -1 \le s \le t \le 1, v \in \Real_+.
\end{equation}
\end{thm}

\begin{proof}
{\bf 1.} Suppose that $a(x, v) \not \equiv a(-x, v)$.
Then there are $\bar{x} \in (-1, 1 )$ and $\bar{v} \in \Real_+$ such that
$$a(\bar{x}, \bar{v}) < a(-\bar{x}, \bar{v}).$$
Therefore, there is $\eps> 0$ such that
$$\bar{x} - \eps \le x \le \bar{x}, \bar{v} \le v \le \bar{v} + \eps \Rightarrow a(x, v) < a(-x, v).$$
Now we introduce the following function:
$$
\left\{     
\begin{aligned}
u(x) &= \bar{v} + \eps, & x \in [-1,\bar{x}-\eps]\\
u(x) &= \bar{v} + \bar{x} - x, & x \in (\bar{x} - \eps, \bar{x})\\
u(x) &= \bar{v}, & x \in [\bar{x}, 1]
\end{aligned}
\right.
$$
Then $u^*(x, v) = u(-x, v)$ and
\begin{multline*}
I(a, u)-I(a, u^*) = \int_{\bar{x}-\eps}^{\bar{x}} F( \bar{v} + \bar{x} - x, a(x, \bar{v} + \bar{x} - x) ) dx -
\int_{-\bar{x}}^{-\bar{x}+\eps} F( \bar{v} + \bar{x} + x, a(x, \bar{v} + \bar{x} + x) ) dx \\ =
\int_{\bar{x}-\eps}^{\bar{x}} ( F( \bar{v} + \bar{x} - x, a(x, \bar{v} + \bar{x} - x) ) -
F( \bar{v} + \bar{x} - x, a(-x, \bar{v} + \bar{x} - x) ) ) dx < 0,
\end{multline*}
which contradicts the assumption. Thus, the first statement is proved.

{\bf 2.} Suppose that the assumption (\ref{almostConcave}) is not satisfied.
Then, by continuity of $a$, there exist $-1 \le s \le t \le 1$, $\eps, \delta> 0$ and $\bar{v} \in \Real_+$, such that
for any $0 \le y \le \eps$ and $\bar{v} \le v \le \bar{v} + \eps$ the following inequality holds:
$$a(s + y, v) + a(t - y, v) + \delta < a( 1 - t + s + 2y, v).$$

Consider the function $u$ (see fig. \ref{uGraph}):
\begin{equation}
\label{parLinU}
\left\{     
\begin{aligned}
u(x) &= \bar{v}, & x \in [-1, s] \cup [t, 1]\\
u(x) &= \bar{v} + x - s, & x \in [s, s + \eps]\\
u(x) &= \bar{v} + \eps, & x \in [s + \eps, t - \eps]\\
u(x) &= \bar{v} + t - x, & x \in [t - \eps, t]
\end{aligned}
\right.
\end{equation}

\begin{center}
\begin{picture}(200,90)
\refstepcounter{pictureCounter}
\label{uGraph}
\put(10,65){\line(1,0){50}}
\put(60,65){\line(1,1){10}}
\put(70,75){\line(1,0){40}}
\put(110,75){\line(1,-1){10}}
\put(120,65){\line(1,0){70}}
\put(0,25){\vector(1,0){200}}
\put(100,15){\vector(0,1){80}}
\put(99,65){\line(1,0){2}}
\put(92,62){$\bar{v}$}
\put(60,24){\line(0,1){2}}
\put(58,14){$s$}
\put(120,24){\line(0,1){2}}
\put(119,14){$t$}
\put(10,24){\line(0,1){2}}
\put(6,14){$-1$}
\put(190,24){\line(0,1){2}}
\put(188,14){$1$}
\put(20,70){$u(x)$}
\put(85,1){Fig. \arabic{pictureCounter}}
\end{picture}
\end{center}
Then
$$
\left\{     
\begin{aligned}
u^*(x) &= \bar{v}, & x \in [-1, 1 - t + s]\\
u^*(x) &= \bar{v} + x - s, & x \in [s, s + \eps]\\
u^*(x) &= \bar{v} + \frac{ x - ( 1 - t + s ) }{2}, & x \in [1 - t + s, 1 - t + s + 2\eps]
\end{aligned}
\right.
$$
(see fig. \ref{uStarGraph}).

\begin{center}
\begin{picture}(200,90)
\refstepcounter{pictureCounter}
\label{uStarGraph}
\put(10,65){\line(1,0){120}}
\put(130,64){\line(2,1){20}}
\put(150,75){\line(1,0){40}}
\put(0,25){\vector(1,0){200}}
\put(100,15){\vector(0,1){80}}
\put(99,65){\line(1,0){2}}
\put(92,67){$\bar{v}$}
\put(130,24){\line(0,1){2}}
\put(110,14){$1 - t + s$}
\put(10,24){\line(0,1){2}}
\put(6,14){$-1$}
\put(190,24){\line(0,1){2}}
\put(188,14){$1$}
\put(20,70){$u^*(x)$}
\put(85,1){Fig. \arabic{pictureCounter}}
\end{picture}
\end{center}

We have
\begin{multline*}
I(a, u^*) = \int_0^{2\eps} F(u(1 - t + s + z), \frac{a(1 - t + s + z, u(1 - t + s + z))}{2}) dz\\
= \int_0^\eps 2 F(\bar{v} + y, \frac{a(1 - t + s + 2y, \bar{v} + y)}{2}) dy\\
0 \le I( a, u ) - I( a, u^* ) =
\int_0^\eps ( F(\bar{v} + y, a(s + y, \bar{v} + y)) + F(\bar{v} + y, a( t - y, \bar{v} + y))\\
- 2 F(\bar{v} + y, \frac{ a(1 - t + s + 2y, \bar{v} + y) }{2})) dy\\
< \int_0^\eps ( F(\bar{v} + y, a(s + y, \bar{v} + y)) + F(\bar{v} + y, a(t - y, \bar{v} + y))\\
- 2 F(\bar{v} + y, \frac{ a(s + y, \bar{v} + y) + a(t - y, \bar{v} + y) + \delta }{2})) dy =: J.
\end{multline*}

Let us consider the function $F(v, p) = p ^ \alpha$.
For $\alpha = 1$, the following inequality trivially holds:
\begin{equation}
\label{anticonvex}
\frac{F(v, p) + F(v, q)}{ 2 } - F(v, \frac{p + q}{ 2 } + \frac{\delta}{ 2}) <0.
\end{equation}
We are interested in $p, q$, lying on a compact $[0 , A]$,
where 
$$A=\max \limits_{(x, v)} a,\qquad (x, v) \in [-1, 1 ] \times u([-1, 1] ).
$$
Therefore, there is an $\alpha> 1$, for which the inequality (\ref{anticonvex})
still holds.
For example, any $1 < \alpha < (\log_2 \frac{ 2 A}{A + \delta})^{-1}$ is suitable.

Thus, we obtain a function $F$ strictly convex with respect to the second argument
for which $J \le 0$. This contradiction proves the second statement.
\end{proof}

\begin{rem}
\label{landesNecessary}
It can be seen that proving the second statement of the theorem
one can replace the function $u$ on the interval $[-1, s]$ by any increasing function.
Thus, in the case where $u$ is pinned at the left end {\rm ($u(-1) = 0$)}
the assumption (\ref{almostConcave}) is also necessary for the inequality (\ref{toprove}) to hold.
\end{rem}

\begin{rem}
If a  non-negative function $a$ is even and concave with respect to the first argument then it satisfies the assumption (\ref{almostConcave}). 
Indeed, for every $s$, $t$ and $u$ we have $a( 1 , u) - a(s, u) \le a(t, u) - a(-1 + t - s, u)$.
Since $a( 1 , u) \ge 0$, we obtain $a(s, u) + a(t, u) \ge a(-1 + t - s, u) = a( 1 - t + s, u)$.
The converse is not true in general, that is not any even
non-negative function satisfying (\ref{almostConcave}) is concave.
\end{rem}

\section{Properties of the weighting function }

For brevity, in this section we omit the second argument of the function $a$.

\begin{lm}
\label{weightSum}
Consider a continuous function $a \ge 0$ defined on $[-1, 1]$
and satisfying the condition (\ref{almostConcave}).
Then for any $-1 \le t_1 \le t_2 \le \ldots \le t_n \le 1$
the following inequalities hold
\begin{align*}
\sum_{k = 1}^n a(t_k) & \ge a( 1 - \sum_{k = 1}^n (-1)^k t_k), & \text{ for even $n$}, & \\
\sum_{k = 1}^n a(t_k) & \ge a(- \sum_{k = 1}^n (-1)^k t_k), & \text{ for odd $n$}. &
\end{align*}
\end{lm}

\begin{proof}
We will prove the lemma by induction.
For $n = 1$ the assertion is trivial.
Now let $n$ be even. Then, by the induction hypothesis,
$$\sum_{k=1}^{n - 1} a(t_k) \ge a( -\sum_{k = 1}^{n - 1} (-1)^k t_k ).$$
Then
$$\sum_{k = 1}^{n - 1} a( t_k ) + a( t_n ) \ge a( -\sum_{k = 1}^{n - 1} (-1)^k t_k ) + a( t_n ) \ge
a( 1 - \sum_{k = 1}^{n} (-1)^k t_k ).$$
In the case of odd $n$ we have the following induction hypothesis:
$$\sum_{k=2}^n a(t_k) \ge a( 1 + \sum_{k = 2}^n (-1)^k t_k ).$$
Then
$$a( t_1 ) + \sum_{k = 2}^n a( t_k ) \ge a( t_1 ) + a( 1 + \sum_{k = 2}^{n} (-1)^k t_k ) \ge
a( -\sum_{k = 2}^{n} (-1)^k t_k + t_1 ) = a( -\sum_{k = 1}^{n} (-1)^k t_k ).$$
\end{proof}

\begin{rem}
Assume that in addition to the conditions of the lemma \ref{weightSum} the function $a$ is even.
Then the following inequalities also hold:
\label{almostConcaveMultRem}
\begin{align*}
\sum_{k = 1}^na(t_k) & \ge a(-1 + \sum_{k = 1}^n (-1)^k t_k), & \text{ for even $n$}, & \\
\sum_{k = 1}^na(t_k) & \ge a(\sum_{k = 1}^n (-1)^k t_k), & \text{ for odd $n$}. &
\end{align*}
\end{rem}

\begin{lm}
\label{periodicity}
{\bf 1.} Let $a$ satisfy $(\ref{almostConcave})$.
If there is $x_0 \in [-1, 1]$, such that $a(x_0) = 0$,
then either $a\Big |_{[x_0, 1]} \equiv 0$
or the set of zeros of $a$ is periodic on $[x_0, 1]$
and the period is a divisor of $1 - x_0$.

{\bf 2.} Let $a$ be even and satisfy $(\ref{almostConcave})$.
If there is $x_0 \in [-1, 1]$, such that $a(x_0) = 0$,
then either $a \equiv 0$
or the function $a$ is periodic on the $[-1, 1]$ interval
and the period is a divisor of $1 - x_0$.
\end{lm}

\begin{proof}
First of all, note that if $a(s) = a(t) = 0$ holds for some $s \le t$
then the inequality (\ref{almostConcave}) implies
$$0 = a(s) + a(t) \ge a( 1 - (t - s) ) \ge 0$$
i.e. $a(1 - (t - s)) = 0$.

Similarly, if $s \le 1 - t$ and $a(s) = a(1 - t) = 0$, then $a(s + t) = 0$.

These two facts imply the following.
If $a(s) = a(t) = 0$ then $a(s + k(t - s)) = 0$ for all positive integers $k$, for which $s + k(t - s) \le 1$.

{\bf 1.}
Substituting $s = t = x_0$, we obtain $a(1) = 0$.

If function $a$ has roots arbitrary close to $x_0$
then it has periodical roots on $[x_0, 1]$ with arbitrary small period.
And thus it vanishes on a set which is dense in $[x_0, 1]$.
By the continuity we have $a\Big |_{[x_0, 1]} = 0$.
Otherwise, let $x_1 > x_0$ be the root of function $a$ closest to $x_0$.
Then there must be a natural number $K$, such that $x_0 + K(x_1 - x_0) = 1$,
otherwise we can find more dense set of roots of $a$.

Suppose now that there exists a root $x_2 > x_0$ of function $a$,
which does not coincide with any of $x_0 + k ( x_1 - x_0 )$ with $k = 0 \dots K$.
Then there exists a root $x_3 \in (1 - (x_1 - x_0), 1)$
and therefore there is a root $x_4 \in (x_0, x_1)$, which leads to a contradiction.

{\bf 2.} The periodicity of zeros of the function $a$ follows from its evenness and from the first assertion of the lemma.
Denote the distance between consecutive zeros by $\Delta$.

Then for $-1 \le x \le 1 - \Delta$ the following holds
$$a(x) = a(x) + a(1 - \Delta) \ge a(x + \Delta).$$

On the other hand, $-1 \le -(x + \Delta) \le 1 - \Delta$, and
$$a(x + \Delta) = a(-(x + \Delta)) + a(1 - \Delta) \ge a(-x) = a(x).$$

Thus, $a(x) = a(x + \Delta)$.
\end{proof}

\begin{lm}
\label{maxSumConcave}
Suppose that $a_1$ and $a_2$ satisfy $(\ref{almostConcave})$.
Then the function $a(x) = \max (a_1(x), a_2(x))$ and $a_1(x) + a_2(x)$ also satisfy $(\ref{almostConcave})$.
\end{lm}
\begin{proof}
\begin{multline*}
a(1 + s + t) = \max(a_1( 1 + s + t), a_2(1 + s + t)) \le
\max(a_1(s) + a_1(t), a_2(s) + a_2(t)) \\
\le \max(a_1(s), a_2(s)) + \max(a_1(t), a_2(t)) =
a(s) + a(t).
\end{multline*}

The second part is obvious.
\end{proof}

\begin{lm}
\label{piecewiseLinearConcave}
Let the function $a$ satisfy $(\ref{almostConcave})$, $k \in \Nat$.
Then a piecewise linear function $a_k$,
interpolating function $a$ using the nodes
$(-1 + \frac{2i}{k})$, $i = 0, 1, \dots, k$,
satisfies $(\ref{almostConcave})$ either.
\end{lm}
\begin{proof}
Let $s = -1 + \frac{2i}{k}$, $t = -1 + \frac{2j}{k}$.
Then the inequality $(\ref{almostConcave})$ holds for $a_k$, because it does for $a$,
and their values at these points are equal.

Now let $s = -1 + \frac{2i}{k}$ and $t \in [-1 + \frac{2j}{k}, -1 + \frac{2(j + 1)}{k}]$.

Consider the linear function $h_1(t) = a_k( 1 - t + s ) - a_k(t) - a_k(s)$.
From already proved it follows that $h_1(-1 + \frac{2j}{k}) \le 0$ and $h_1(-1 + \frac{2(j + 1)}{k}) \le 0$.
While $h_1$ is linear, $h_1(t) \le 0$.
Thus, the inequality holds for every $s \in -1 + \frac{2i}{k}$ and $t \in [-1, 1]$.

Consider the function $h_2(y) = a_k(\frac{2j}{k}) - a_k(s - y) - a_k(t + y)$, where $1 - t + s = \frac{2j}{k}$.
Suppose, $s + y_0$ is one of the interpolation nodes, then $t + y_0$ is also an interpolation node.
Thereby, $h_2(y_0) = a(\frac{2j}{k}) - a(s - y) - a(t + y) \le 0$.
Between such $y_0$ the $h_2$ function is linear.
Also the boundary points of the domain of $h_2$ are nodes of interpolation.
Therefore $h_2(y) \le 0$ on its entire domain.

Consider the function $h_3(s) = a_k( 1 - t + s ) - a_k(t) - a_k(s)$ for any fixed $t \in [-1, 1]$.
This function is piecewise linear,
and it can bend at each $s$, which is an interpolation node itself of for which
$1 - t + s$ is an interpolation node.
However, we have already proved that at these points $h_3(s) \le 0$.
The boundary points of the domain of $h_3$ are the nodes of interpolation, thus, $h_3(s) \le 0$ everywhere.
\end{proof}


\begin{thebibliography}{99}
\bibitem{ASC} G.~Alberti,~F.~Serra~Cassano: Non-occurrence of gap for one-dimentional autonomous functionals,
Proceedings of ``Calc. Var., Homogen. and Cont. Mech.'', G.~Bouchitt\'e, G.~Buttazzo, P.~Suquet, ed.: World Sci., Singapore, p.~1--17, 1994
\bibitem{Br} F.~Brock: Weighted Dirichlet-type inequalities for Steiner symmetrization,
Calc. Var. and PDEs~{\bf 8}, p.~15--25, 1999
\bibitem{Kawohl} B.~Kawohl: Rearrangements and convexity of level sets in PDE,
Lecture notes in mathematics {\bf 1150}. Berlin; Springer Verlag, 1985. 134~p.
\bibitem{Lan} R.~Landes: Some remarks on rearrangements and functionals with non-constant density,
Math.~Nachr.~{\bf 280}, \No5--6, p.~560--570, 2007
\bibitem{DAN} С.~Банкевич, А.~Назаров: Об обобщении неравенства Пойа-Сеге для одномерных функционалов,
Доклады Академии Наук~{\bf 438}, \No1, с.~11--13, 2011
\bibitem{BGH} Дж.~Буттаццо, М.~Джаквинта, С.~Гильдебрандт: Одномерные вариационные задачи. Введение,
Научная книга, Новосибирск, 2002. 246~с.
%G.~Buttazzo, M.~Giaquinta, S.~Hildebrandt: One-dimensional Variational Problems,
%Oxford Lecture Series in Mathematics and Its Applications {\bf 15}, 1998. 272 p.
\bibitem{Zh1} В.~В.~Жиков: О весовых соболевских пространствах,
Матем. сб., {\bf 189}, \No8, с.~27--58, 1998
\bibitem{Zh2} В.~В.~Жиков: К проблеме предельного перехода в дивергентных неравномерно эллиптических уравнениях,
Функц. анализ и его прил., {\bf 35}, \No1, с.~23--39, 2001
\bibitem{LL} Э.~Либ, М.~Лосс: Анализ, Научная книга, Новосибирск, 1998. 276~с.
\bibitem{Fed} Г.~Федерер: Геометрическая теория меры, Наука, М., 1987. 760~с.

\end{thebibliography}

\end{document}
