\section{Appendix . The case of symmetric permutation}

\subsection{Prerequisites for weight}

\begin{lm}
If the inequality $(\ref{toproveSymm})$ holds for any $F \in \mathfrak{F}$
and arbitrary piecewise linear $u$, then
weight $a$ satisfies
\begin{equation}
\label{almostConvex}
\forall s, t \in [-1, 1], \forall v \in \Real_+ \quad
a( s, v ) + a( t, v ) \ge a\Big( \frac{ s - t }{2}, v \Big) + a\Big( \frac{ t - s }{2}, v \Big).
\end{equation}
\end{lm}

\begin{proof}
Assume that the inequality (\ref{almostConvex}) is not satisfied.
Then there are $-1 \le s < t \le 1$, $\eps, \delta > 0$ ($2 \eps < t - s$) and $\bar{v} \in \Real_+$,
such that for any $0 \le z \le \eps$ and any $\bar{v} \le v \le \bar{v} + \eps$ satisfied
\begin{equation}
\label{notConvex}
a(s + z, v + z) + a(t - z, v + z) + 2 \delta < a\Big(\frac{s - t}{2} + z, v + z \Big) + a\Big(\frac{t - s}{2} - z, v + z \Big).
\end{equation}

Consider the function $u$, introduced in (\ref{parLinU}). then
$$
\left\{
\begin{aligned}
\bar{u}(x) &= \bar{v}, & x \in &[-1, \frac{s - t}{2}] \cup [\frac{t - s}{2}, 1]\\
\bar{u}(x) &= \bar{v} + x - \frac{s - t}{2}, & x \in &[\frac{s - t}{2}, \frac{s - t}{2} + \eps]\\
\bar{u}(x) &= \bar{v} + \eps, & x \in &[\frac{s - t}{2} + \eps, \frac{t - s}{2} - \eps]\\
\bar{u}(x) &= \bar{v} + \frac{t - s}{2} - x, & x \in &[\frac{t - s}{2} - \eps, \frac{t - s}{2}].
\end{aligned}
\right.
$$

Hence we obtain
\begin{multline*}
0 \le I(a, u) - I(a, \overline{u}) \\
=\int_0^{\eps} F( u(s + z), \frac{a( s + z, u(s + z) )}{\eps} ) dz + \int_0^{\eps} F( u(t - z), \frac{a(t - z, u(t - z))}{\eps} ) dz \\
-\int_0^{\eps} F( \bar{u}(\frac{s - t}{2} + z), \frac{a( \frac{s - t}{2} + z, \bar{u}(\frac{s - t}{2} + z) )}{\eps} ) dz \\
-\int_0^{\eps} F( \bar{u}(\frac{t - s}{2} - z), \frac{a( \frac{t - s}{2} - z, \bar{u}(\frac{t - s}{2} - z) )}{\eps} ) dz =: J.
\end{multline*}

Take $F(v, p) := f(p) := p + \gamma p^2$, where $\gamma > 0$.
then
\begin{multline*}
J = \int_0^{\eps} \big( f(\frac{a(s + z, \bar{v} + z)}{\eps}) + f(\frac{a(t - z, \bar{v} + z)}{\eps}) \\
- f(\frac{a(\frac{s - t}{2} + z, \bar{v} + z)}{\eps}) - f(\frac{a(\frac{t - s}{2} - z, \bar{v} + z)}{\eps}) \big) dz.
\end{multline*}

We denote $A := \max a(x, v)$, where the maximum is taken over all $x \in [-1, 1]$ and $v \in [\bar{v}, \bar{v} + \eps]$.
If you take the $\gamma := \frac{\delta / \eps}{(A / \eps)^2} > 0$ ,
then for $p \le \frac{A}{\eps}$ , we have $p \le f( p ) \le p + \frac{\delta}{\eps}$, and
\begin{equation*}
J \le \frac{1}{\eps} \int_0^{\eps} \big( a(s + z, \bar{v} + z) + a(t - z, \bar{v} + z) + 2 \delta
- a(\frac{s - t}{2} + z, \bar{v} + z) - a(\frac{t - s}{2} - z, \bar{v} + z) \big) dz < 0
\end{equation*}
(the last inequality follows from (\ref{notConvex})).

Thus , we arrive at a contradiction , which completes the proof .
\end{proof}

\begin{lm}
If the function $a \in C([-1, 1] \times \Real_+)$ the relation $(\ref{almostConvex})$,
it is even and convex in the first argument .
\end{lm}

\begin{proof}
Assume for the moment that $a(\cdot, v) \in C^1([-1, 1])$ for each $v$.
We fix arbitrary $s \in [-1, 1]$ and $v \in \Real_+$ and consider the function
$$b(x) := a( s, v ) + a( x, v ) - a( \frac{ s - x }{2}, v ) - a( \frac{ x - s }{2}, v ) \ge 0.$$
$x = -s$ is the minimum point of $b$, since $b(-s) = 0$.
hence,
$$b'(-s) = a'_x( -s, v ) + \frac{1}{2} a'_x( s, v ) - \frac{1}{2} a'_x( -s, v ) = 0,$$
ie $a'_x( s, v ) = -a'_x( -s, v )$. Thus, the function $a(\cdot, v)$ is even.

Now consider the case of a continuous $a$.

We extend $a( x, v ) := a( -1, v )$ with $x < -1$ and $a( x, v ) := a( 1, v )$ with $x > 1$ .
Consider the average of the function :
$$a_\rho( x, v ) = \int_\Real \omega_\rho ( z ) a( x - z, v ) dz = \int_\Real \omega_\rho ( z ) a( x + z, v ) dz,$$
where $\omega_\rho(z)$ --- averaging kernel with radius $\rho$.
then
\begin{multline*}
a_\rho( s, v ) + a_\rho( t, v ) - a_\rho( \frac{ s - t }{2}, v ) - a_\rho( \frac{ t - s }{2}, v ) =
\\ \int_\Real \omega_\rho ( z ) \big( a( s - z, v ) + a( t + z, v ) - a( \frac{ s - t }{2} - z, v ) - a( \frac{ t - s }{2} + z, v ) \big) dz \ge 0.
\end{multline*}
So $a_\rho(\cdot, v)$ --- even.
Passing to the limit as $\rho \to 0$ , we obtain that $a(\cdot, v)$ --- even.

Finally, for any $s$, $t$ and $v$ , we have
$$a( s, v ) + a( t, v ) = a( s, v ) + a( -t, v ) \ge 2 a\big( \frac{ s + t }{2}, v \big).$$
\end{proof}

